Substituting the definition of $r_\pi$ into equation~\ref{eq:kclEmitter}:

\begin{subequations}
\begin{align}
\frac{(v_e - v_b)g_m}{\beta} - g_m(v_b - v_e) + \frac{v_e}{R_{e2}} &= 0\\
g_m \left( \frac{v_e - v_b}{\beta} + (v_e - v_b) \right) + \frac{v_e}{R_{e2}} &= 0\\
g_m (v_e - v_b) \left( \frac{1}{\beta} + 1 \right) + \frac{v_e}{R_{e2}} &= 0 \label{eq:kclEmitter2}
\end{align}
\end{subequations}

Equating equations \ref{eq:kclEmitter2} and \ref{eq:kclCollector}:

\begin{subequations}
\begin{align}
g_m (v_e - v_b) \left( \frac{1}{\beta} + 1 \right) + \frac{v_e}{R_{e2}} &= \frac{v_c}{R_c} + g_m(v_b - v_e)\\
g_m (v_e - v_b) \left( \frac{1}{\beta} + 2 \right) + \frac{v_e}{R_{e2}} &= \frac{v_c}{R_c} \label{eq:emitterEqCollector}
\end{align}
\end{subequations}

By Ohm's law:

\begin{subequations}
\begin{align}
v_e &= i_e R_{e2}\\
&= R_{e2} (i_b + i_c)\\
&= R_{e2} (i_b + \beta i_b)\\
&= R_{e2} i_b (\beta + 1) \label{eq:v_e}
\end{align}
\end{subequations}

\begin{subequations}
\begin{align}
v_b - v_e &= r_\pi i_b\\
\therefore v_b - R_{e2} i_b (\beta + 1) &= r_\pi i_b
\end{align}
\end{subequations}

\begin{subequations}
\begin{align}
v_c &= -i_c R_c\\
&= -\beta i_b R_c \label{eq:v_c}
\end{align}
\end{subequations}

Substituting equation \ref{eq:v_e} into \ref{eq:emitterEqCollector}

\begin{subequations}
\begin{align}
g_m \left(R_{e2} i_b (\beta + 1) - v_b\right) \left( \frac{1}{\beta} + 2 \right) + i_b (\beta + 1) &= \frac{v_c}{R_c}
\end{align}
\end{subequations}